src/ASN1/ASN1.Spec.Interpreter.fst
@@ -2,6 +2,8 @@ module ASN1.Spec.Interpreter
 
 include LowParse.Spec.Base
 include LowParse.Spec.Combinators
+include LowParse.Spec.List
+include LowParse.Spec.Defaultable
 
 open ASN1.Base
 open ASN1.Spec.Content.BOOLEAN
@@ -16,8 +18,65 @@ open ASN1.Spec.Content.OIDU32
 open ASN1.Spec.ILC
 open ASN1.Spec.Choice
 open ASN1.Spec.Sequence
+open ASN1.Spec.Any
 
 module List = FStar.List.Tot
+
+let generate_defaultable_item (item : asn1_gen_item_k) :
+  Tot (option (asn1_decorated_t item))
+= match item with
+  | (| _, _, dk |) -> match dk with
+                       | ASN1_PLAIN_ILC k -> None
+                       | ASN1_OPTION_ILC k -> Some (None #(asn1_t k)) 
+                       | ASN1_DEFAULT_TERMINAL id #k defv -> Some (Default #(asn1_terminal_t k) #defv)
+
+let asn1_decorated_item_as_parser_aux (item : asn1_gen_item_k) (p : asn1_strong_parser (asn1_decorated_pure_t item)) :
+  Tot (asn1_strong_parser (asn1_decorated_t item))
+= match item with
+  | (| _, _, dk|) ->
+         match dk with
+         | ASN1_PLAIN_ILC _ -> p
+         | ASN1_OPTION_ILC _ -> p `parse_synth` (Some)
+         | ASN1_DEFAULT_TERMINAL _ defaultv ->
+                    ((p
+                    `parse_filter`
+                    (defaultv_filter defaultv))
+                    `parse_synth`
+                    (defaultv_synth defaultv))
+
+let asn1_decorated_item_as_parser_aux_non_default
+  (item : asn1_gen_item_k)
+  (p : asn1_strong_parser (asn1_decorated_pure_t item))
+  (input : bytes)
+: Lemma
+  (ensures (parse_defaultable_injective_cond (generate_defaultable_item item) (asn1_decorated_item_as_parser_aux item p) input))
+= let p' = (asn1_decorated_item_as_parser_aux item p) in
+  match item with
+  | (| _, _, dk|) ->
+        match dk with
+        | ASN1_PLAIN_ILC _ -> _
+        | ASN1_OPTION_ILC _ -> 
+          let defv = generate_defaultable_item item in
+          (match parse p' input with
+           | None -> ()
+           | Some (v, _) -> 
+             let _ = parse_synth_eq p (Some) input in
+             assert (Some? #(asn1_decorated_pure_t item) v);
+             ())
+        | ASN1_DEFAULT_TERMINAL _ defaultv ->
+          let defv = generate_defaultable_item item in
+          (match parse p' input with
+           | None -> ()
+           | Some (v, _) -> 
+             let _ = parse_synth_eq (p `parse_filter` (defaultv_filter defaultv)) (defaultv_synth defaultv) input in
+             ())
+
+let asn1_decorated_item_as_weak_parser
+  (item : asn1_gen_item_k)
+  (p : asn1_strong_parser (asn1_decorated_pure_t item))
+: asn1_weak_parser (asn1_decorated_t item)
+= let _ = Classical.forall_intro (asn1_decorated_item_as_parser_aux_non_default item p) in
+  parse_defaultable (generate_defaultable_item item) (asn1_decorated_item_as_parser_aux item p)
 
 let rec asn1_terminal_as_parser (k : asn1_terminal_k) : asn1_weak_parser (asn1_terminal_t k)  =
   match k with
@@ -37,13 +96,28 @@ and asn1_content_as_parser (k : asn1_content_k) : Tot (asn1_weak_parser (asn1_co
   match k with
   | ASN1_TERMINAL k' -> asn1_terminal_as_parser k'
   | ASN1_SEQUENCE items pf -> make_asn1_sequence_parser (asn1_sequence_as_parser items)
-  | ASN1_SEQUENCE_OF k' -> fail_parser _ _ (* admit Seq.seq (asn1_t k') *)
+  | ASN1_SEQUENCE_OF k' -> weaken asn1_weak_parser_kind (parse_list (asn1_as_parser k'))
   | ASN1_SET_OF k' -> weaken _ (asn1_as_parser k')
   | ASN1_PREFIXED k' -> weaken _ (asn1_as_parser k')
-  | ASN1_ANY_OID ls pf -> fail_parser _ _ (* admit *)
-  | ASN1_ANY_INTEGER ls pf -> fail_parser _ _ (* admit *)
+  | ASN1_ANY_OID id ls pf -> make_asn1_any_OIDU32_parser id ls pf k (asn1_ls_as_parser asn1_oid_t ls)
+  | ASN1_ANY_INTEGER id ls pf -> make_asn1_any_INTEGER_parser id ls pf k (asn1_ls_as_parser asn1_integer_t ls)
 
-and asn1_lc_as_parser (lc : list (asn1_id_t & asn1_content_k)) : Tot (lp : list (asn1_id_t & gen_parser) {asn1_lc_t lc == extract_types lp})  (decreases lc) =
+and asn1_ls_as_parser (t : eqtype) (ls : list (t * asn1_gen_item_k)) : Tot (lp : list (t & (gen_parser asn1_weak_parser_kind)) {asn1_any_t t ls == extract_types lp}) (decreases ls) =
+  match ls with
+  | [] -> [] 
+  | h :: tl -> 
+    let (x, y) = h in
+    let yp = match y with
+             | (| _, _, dk |) -> match dk with
+                                | ASN1_PLAIN_ILC k -> asn1_as_parser k
+                                | ASN1_OPTION_ILC k -> asn1_as_parser k
+                                | ASN1_DEFAULT_TERMINAL id #k defv ->
+                                  let p = asn1_terminal_as_parser k in
+                                  (parse_asn1_ILC id #(ASN1_TERMINAL k) p)
+    in                              
+    (x, Mkgenparser _ (asn1_decorated_item_as_weak_parser y yp)) :: (asn1_ls_as_parser t tl)
+
+and asn1_lc_as_parser (lc : list (asn1_id_t & asn1_content_k)) : Tot (lp : list (asn1_id_t & (gen_parser asn1_strong_parser_kind)) {asn1_lc_t lc == extract_types lp})  (decreases lc) =
   match lc with
   | [] -> [] 
   | h :: t -> 
@@ -66,7 +140,7 @@ and asn1_as_parser_twin (#s : _) (k : asn1_k s) : Tot (asn1_strong_parser (asn1_
     let _ = make_asn1_choice_parser_twin_cases_injective lc pf k lp in
     (make_asn1_choice_parser lc pf k lp, make_asn1_choice_parser_twin lc pf k lp)
 
-and asn1_decorated_as_parser (item : asn1_gen_item_k) : Tot (gp : gen_decorated_parser_twin {Mkgendcparser?.d gp == item}) =
+and asn1_decorated_as_parser_twin (item : asn1_gen_item_k) : Tot (gp : gen_decorated_parser_twin {Mkgendcparser?.d gp == item}) =
   match item with
   | (| _, _, dk |) -> match dk with
                     | ASN1_PLAIN_ILC k -> 
@@ -82,5 +156,5 @@ and asn1_decorated_as_parser (item : asn1_gen_item_k) : Tot (gp : gen_decorated_
 and asn1_sequence_as_parser (items : list asn1_gen_item_k) : Tot (lp : list gen_decorated_parser_twin {List.map (Mkgendcparser?.d) lp == items}) (decreases items) =
   match items with
   | [] -> []
-  | hd :: tl -> (asn1_decorated_as_parser hd) :: (asn1_sequence_as_parser tl)
+  | hd :: tl -> (asn1_decorated_as_parser_twin hd) :: (asn1_sequence_as_parser tl)
   
